language/pure_configScript.sml
@@ -4,23 +4,8 @@ open arithmeticTheory integerTheory stringTheory optionTheory;
 
 val _ = new_theory "pure_config";
 
-(* Configuration record for the parametric atoms.
-   parAtomOp:
-     It takes an element of type 'a (from AtomOp) and returns a
-     function that takes a "'b list" element and SOME b if the
-     number of arguments is correct, NONE otherwise
-*)
-
-Datatype:
-  conf = <| parAtomOp  : 'a -> 'b list -> 'b option; |>
-End
-
-(*
- * Assume an abstract configuration exists.
- *)
-
 val atom_op_ty = new_type ("atom_op", 0);
 val atom_lit_ty = new_type ("lit", 0);
-val the_config = new_constant ("config", “:(atom_op, lit) conf”);
+val the_config = new_constant ("eval_op", “:atom_op -> lit list -> (lit + bool) option”);
 
 val _ = export_theory ();
